src/LocalReasoning.v
@@ -2,8 +2,8 @@
 (* Clément Blaudeau - Lamp@EPFL 2021 *)
 (** This file defines the main result of local reasoning, built upon wellformedness, compatibility, scopability and stackability. In a wellformed, fully initialized context, a newly created object can only access hot (transitively fully initialized) locations. *)
 
-From Celsius Require Export Scopability Compatibility PartialMonotonicity Stackability.
-Require Import ssreflect ssrbool Psatz Sets.Ensembles List.
+From Celsius Require Export Scopability Compatibility PartialMonotonicity Stackability MetaTheory.
+Require Import ssreflect ssrbool Psatz Sets.Ensembles List Coq.Sets.Finite_sets_facts.
 Import ListNotations.
 Open Scope nat_scope.
 
@@ -51,4 +51,135 @@ Proof.
       eauto using stk_theorem with pM stk cmpt wf lia.
     eapply scopability_theorem in H; eauto with pM wf lia; steps.
   + eapply H3; eauto using In_singleton.
+Qed.
+
+
+
+(** ** Local reasoning *)
+Parameter reachabilityb : Store -> Loc -> Loc -> bool.
+Parameter reachability_refl: forall σ l l', Bool.reflect (reachability σ l l') (reachabilityb σ l l').
+
+Lemma reachabilityb_true:
+  forall σ l l',
+    (σ ⊨ l ⇝ l') <-> (reachabilityb σ l l' = true).
+Proof.
+  intros.
+  destruct (reachability_refl σ l l'); steps.
+Qed.
+
+Lemma reachabilityb_false:
+  forall σ l l',
+    (~ (σ ⊨ l ⇝ l')) <-> (reachabilityb σ l l' = false).
+Proof.
+  intros.
+  destruct (reachability_refl σ l l'); steps.
+Qed.
+
+Lemma synchronization: forall Σ σ (l: Loc),
+    wf σ ->
+    Σ ⊨ σ ->
+    (forall (l': Loc), σ ⊨ l ⇝ l' -> Σ ⊨ l' : warm) ->
+    exists Σ',
+      (Σ' ⊨ σ) /\
+        Σ ≼ Σ' /\
+        Σ ▷ Σ' /\
+        Σ ≪ Σ' /\
+        (forall (l': Loc), σ ⊨ l ⇝ l' -> Σ' ⊨ l' : hot).
+Proof with (meta; eauto with typ).
+  intros Σ σ l H__wf H__st; intros.
+  remember ((fun l' '(C,μ) => if (reachabilityb σ l l') then (C, hot) else (C, μ)):Loc -> Tpe -> Tpe) as f.
+  remember (map (fun '(l, T) => (l, f l T)) Σ) as Σ'.
+  exists Σ'.
+  assert (Hyp: forall (A B C D E: Prop), ((D -> B -> A) /\ B /\ C /\ D /\ E) -> (A /\ B /\ C /\ D /\ E)) by firstorder.
+  apply Hyp. clear Hyp.
+  repeat split.
+  - intros H__stk H__mn l' H__l'. rewrite HeqΣ' in H__l'.
+    apply in_dom_map in H__l'...
+    specialize (H__st l' H__l') as [C [ω [μ [? [? ?] ]]]] ...
+    destruct (reachability_refl σ l l'); steps.
+    + pose proof (H _  r) ...
+      exists C0, ω, hot; repeat split => //.
+      * apply reachabilityb_true in r.
+        erewrite getType_map; steps; eauto.
+        inverts matched. reflexivity.
+      * inverts H4; meta; eauto with typ.
+        apply ot_hot; intros f v H__val.
+        assert (σ ⊨ l ⇝ v) by eauto with rch.
+        assert (Σ ⊨ v : warm) by eauto.
+        inverts H4. inverts H6 ...
+        exists x, (x, hot) ...
+        erewrite getType_map ...
+        destruct (reachability_refl σ l v); steps.
+    + exists C, ω, μ; repeat split => // ...
+      erewrite getType_map ...
+      destruct (reachability_refl σ l l'); steps.
+  - intros l' H__l'.
+    destruct (getType Σ l') as [T1 |] eqn:?; [|exfalso; apply getType_none in Heqo; eauto].
+    exists T1. subst.
+    erewrite getType_map; eauto. steps; eexists; steps.
+  - intros l' C Ω H__l'.
+    erewrite HeqΣ', getType_map; eauto. steps.
+    destruct (reachability_refl σ l l'); steps.
+    apply H in r.
+    inverts r.
+    inverts H0 ...
+    inverts H4.
+  - intros l' H__l'.
+    right.
+    destruct (getType (map (fun '(l, T) => (l, f l T)) Σ) l')
+      as [[C μ] |] eqn:?; [| eapply getType_none in Heqo; steps].
+    eapply getType_in_dom_map; eauto.
+  - intros l' H__rch.
+    specialize (H l' H__rch) as [C H0].
+    exists C, (C, hot); eauto with typ.
+    inverts H0; meta.
+    erewrite HeqΣ', getType_map; eauto. steps.
+    destruct (reachability_refl σ l l'); steps.
+Qed.
+
+
+
+
+Lemma local_reasoning2: forall Σ1 Σ2 σ1 σ2 (L1 L2: LocSet),
+    L1 ⪽ σ1 ->
+    L2 ⪽ σ2 ->
+    (σ1, L1) ⋖ (σ2, L2) ->
+    (Σ1 ≪ Σ2) ->
+    (Σ1 ▷ Σ2) ->
+    (Σ1 ≼ Σ2) ->
+    (Σ1 ⊨ σ1) ->
+    (Σ2 ⊨ σ2) ->
+    (Σ1 ⊨ L1 : hot) ->
+    wf σ2 ->
+    exists Σ', (Σ1 ≪ Σ') /\
+            (Σ1 ≼ Σ') /\
+            (Σ1 ▷ Σ') /\
+            (Σ' ⊨ σ2) /\
+            (Σ' ⊨ L2 : hot).
+Proof.
+  intros Σ1 Σ2 σ1 σ2 L1 L2 H1 H2.
+  pose proof (storeSubset_finite _ _ H2).
+  gen Σ1 Σ2 σ1 σ2 L1.
+  eapply finite_sets_ind with (F := L2); eauto; intros.
+  - exists Σ2; steps.
+    intros l Hl. inversion Hl.
+  - clear H L2. rename F into L2, a into l2.
+    unfold Add in *.
+    assert ((σ1, L1) ⋖ (σ2, L2)) by eauto with scp.
+    pose proof (storeSubset_union_l _ _ _ H2).
+    specialize (H1 Σ1 Σ2 σ1 σ2 H12 L1 H3 H H5 H6 H7 H8 H9 H10) as [Σ2' [ ]]; steps.
+    clear Σ2 H5 H6 H7 H9.
+    pose proof (synchronization Σ2' σ2 l2 H11 H15) as [Σ'' [ ]] ; steps.
+    + assert (l' < dom σ1 \/ l' >= dom σ1) as [|] by lia.
+      * specialize (H4 H3 H2 l' H6) as[l1 [H__l1 H__rch1]];[ exists l2; split; eauto with wf |].
+        specialize (H10 l1 H__l1).
+        lets: hot_transitivity  H10 H8 H__rch1.
+        specialize (H14 l').
+        meta; steps; meta; eauto with typ.
+        exists C. eapply vt_sub; eauto with typ.
+      * specialize (H1 l') as [ ]; eauto.
+        -- assert (in_dom Σ2' l2) by admit.
+        -- specialize (H8 l' H1); steps. apply getObj_dom in H8. lia.
+    + exists Σ''; repeat split; eauto with typ.
+      intros l0 [ l2' | ]; try inSingleton; eauto with rch wf typ.
 Qed.
